scaffolding for an is_non_informative API

src/tactics/FStar.Tactics.Types.fst
@@ -111,6 +111,7 @@ let get_phi (g:goal) : option term =
 let is_irrelevant (g:goal) : bool =
     Option.isSome (get_phi g)
 
+let non_informative_token (g:env) (t:typ) = unit
 let subtyping_token (g:env) (t0 t1:typ) = unit
 let equiv_token (g:env) (t0 t1:typ) = unit
 let typing_token (g:env) (e:term) (c:Core.tot_or_ghost & typ) = unit
