ulib/FStar.Tactics.Types.fsti
@@ -61,6 +61,7 @@ type guard_policy =
     | Drop      // Drop guards, clearly unsound! careful!
 
 (* Typing reflection *)
+val non_informative_token (g:env) (t:typ) : Type0
 val subtyping_token (g:env) (t0 t1:typ) : Type0
 val equiv_token (g:env) (t0 t1:typ) : Type0
 val typing_token (g:env) (e:term) (c:tot_or_ghost & typ) : Type0
